several implementation of the loop in generate

specs/HMAC_DRBG_generate_algorithm.v
@@ -4,13 +4,27 @@ Require Import List. Import ListNotations.
 Require Import DRBG_working_state.
 Require Import HMAC_DRBG_update.
 Require Import DRBG_generate_algorithm_result.
-Require Import floyd.sublist.
 
-Function HMAC_DRBG_generate_helper (HMAC: list Z -> list Z -> list Z) (key v: list Z) (requested_number_of_bytes: Z) {measure Z.to_nat requested_number_of_bytes}: (list Z * list Z) :=
+Function HMAC_DRBG_generate_helper (HMAC: list Z -> list Z -> list Z) (key v: list Z) (requested_number_of_bytes: nat) {measure (fun x => x) requested_number_of_bytes}: (list Z * list Z) :=
+  match requested_number_of_bytes with
+    | O => (v, [])
+    | _ => 
+    let len := 32%nat in (* TODO get this from property of HMAC *)
+    let (v, rest) := HMAC_DRBG_generate_helper HMAC key v (requested_number_of_bytes - 32)%nat in
+    let v := HMAC v key in
+    let temp := v in
+    (v, rest ++ temp)
+  end. 
+Proof.
+  intros.
+  omega.
+Defined.
+
+Function HMAC_DRBG_generate_helper_Z (HMAC: list Z -> list Z -> list Z) (key v: list Z) (requested_number_of_bytes: Z) {measure Z.to_nat requested_number_of_bytes}: (list Z * list Z) :=
   if Z.geb 0 requested_number_of_bytes then (v, [])
   else
     let len := 32%nat in (* TODO get this from property of HMAC *)
-    let (v, rest) := HMAC_DRBG_generate_helper HMAC key v (requested_number_of_bytes - (Z.of_nat len)) in
+    let (v, rest) := HMAC_DRBG_generate_helper_Z HMAC key v (requested_number_of_bytes - (Z.of_nat len)) in
     let v := HMAC v key in
     let temp := v in
     (v, rest ++ temp). 
@@ -28,6 +42,42 @@ Proof.
   apply Z2Nat.inj_lt in H; omega.
 Defined.
 
+Fixpoint HMAC_DRBG_generate_helper_rounds (HMAC: list Z -> list Z -> list Z) (key v: list Z) (rounds: nat): (list Z * list Z) :=
+  match rounds with
+    | O => (v, [])
+    | S rounds' => 
+    let (v, rest) := HMAC_DRBG_generate_helper_rounds HMAC key v rounds' in
+    let v := HMAC v key in
+    let temp := v in
+    (v, rest ++ temp)
+  end.
+
+Fixpoint HMAC_v_n_times (HMAC: list Z -> list Z -> list Z) key v n :=
+  match n with
+    | O => v
+    | S n' =>
+      let v' := HMAC_v_n_times HMAC key v n' in
+      HMAC v' key
+  end
+.
+
+Lemma HMAC_DRBG_generate_helper_rounds_v:
+  forall HMAC key v v' n b,
+    (v', b) = HMAC_DRBG_generate_helper_rounds HMAC key v n ->
+    v' = HMAC_v_n_times HMAC key v n.
+Proof.
+  intros until n.
+  revert HMAC key v v'.
+  induction n as [|n']; intros. simpl in H. inv H. reflexivity.
+  simpl in H.
+  simpl.
+  remember (HMAC_DRBG_generate_helper_rounds HMAC key v n') as x; destruct x.
+  apply IHn' in Heqx.
+  subst.
+  inv H.
+  reflexivity.
+Qed.
+
 Definition HMAC_DRBG_generate_algorithm (HMAC: list Z -> list Z -> list Z) (reseed_interval: Z) (working_state: DRBG_working_state) (requested_number_of_bytes: Z) (additional_input: list Z): DRBG_generate_algorithm_result :=
   let '(v, key, reseed_counter) := working_state in
   if Z.gtb reseed_counter reseed_interval then generate_algorithm_reseed_required
@@ -36,8 +86,8 @@ Definition HMAC_DRBG_generate_algorithm (HMAC: list Z -> list Z -> list Z) (rese
                       | [] => (key, v)
                       | _::_ => HMAC_DRBG_update HMAC additional_input key v
                     end in
-    let (v, temp) := HMAC_DRBG_generate_helper HMAC key v requested_number_of_bytes in
-    let returned_bits := sublist 0 requested_number_of_bytes temp in
+    let (v, temp) := HMAC_DRBG_generate_helper_Z HMAC key v requested_number_of_bytes in
+    let returned_bits := firstn (Z.to_nat requested_number_of_bytes) temp in
     let (key, v) := HMAC_DRBG_update HMAC additional_input key v in
     let reseed_counter := reseed_counter + 1 in
     generate_algorithm_success returned_bits (v, key, reseed_counter).      
